ESPL: More useful premise for match step typing

data/isabelle/src/ESPLogic/WeakTyping.thy
@@ -293,6 +293,39 @@ next
     using varOfRecv by (auto intro!: typ_rule thread_exists)
 qed
 
+(* TODO ? *)
+definition typing_A_ext :: "typing \<Rightarrow> (role \<times> varid) \<Rightarrow> msgtype"
+where "typing_A_ext typing rv \<equiv> case rv of
+    (r, MVar n) \<Rightarrow> typing (r, n)
+  | (_, AVar _) \<Rightarrow> AgentT"
+
+declare typing_A_ext_def[simp]
+
+lemma (in reachable_thread) matchEq_typed:
+  assumes approx: "(t,r,s) \<in> approx typing"
+  and todo_step: "todo = step # todo'"
+  and "matchEqStep step"
+  shows "s (matchVar step, i) \<in> typing_A_ext typing (done@todo, matchVar step) i (t,r,s)"
+proof -
+  obtain lbl v pt where match: "step = Match lbl True v pt"
+    using `matchEqStep step` by (auto dest!: matchEqStepD)
+  thus ?thesis proof (cases v, simp)
+    case (MVar n) note mcase = this
+    hence "n \<in> used_vars step" using match by auto
+    then obtain sstep where "n \<in> sourced_vars sstep" and sstep: "(i, sstep) \<in> steps t"
+      using todo_step thread_exists by (auto dest: source_step)
+    hence sources: "MVar n \<in> FV_rolestep sstep" by auto
+    have "s (MVar n, i) \<in> typing (done@todo, n) i (t,r,s)"
+      using sstep thread_exists sources approx
+      apply -
+      apply (drule in_approxD, simp)
+      apply (rule roleMap_SomeI)
+      apply (auto)
+      done
+    thus ?thesis using match mcase by simp
+  qed
+qed
+
 lemma (in reachable_state) reachable_in_approxI:
   assumes monoTyp: "monoTyp typing"
   and source_case:
@@ -309,8 +342,9 @@ lemma (in reachable_state) reachable_in_approxI:
        (t,r,s) \<in> approx typing;
        r i = Some (done, step # todo, skipped);
        
-       recvStep step    \<Longrightarrow> Some m = inst s i (stepPat step) \<and> m \<in> knows t;
-       matchEqStep step \<Longrightarrow> Some (s (matchVar step, i)) = inst s i (stepPat step)
+       recvStep step \<Longrightarrow> Some m = inst s i (stepPat step) \<and> m \<in> knows t;
+       matchEqStep step \<Longrightarrow>
+         the (inst s i (stepPat step)) \<in> typing_A_ext typing (R, matchVar step) i (t,r,s)
      \<rbrakk> \<Longrightarrow> 
         s (MV n i) \<in> typing (R, n) i (t @ [Step (i, step)], r(i \<mapsto> (done @ [step], todo, skipped)), s)"
   shows "(t,r,s) \<in> approx typing"
@@ -538,6 +572,9 @@ proof -
                   apply(rule source_case)
                   apply(simp_all add: th1.role_in_P th1.roleMap th1.thread_exists
                                       in_set_splits_conv remove_hints)
+                  apply(drule th1.matchEq_typed)
+                  apply(auto)
+                  apply(metis the.simps)
                   done
             qed
           qed
@@ -575,7 +612,7 @@ text{*
 *}
 lemma (in reachable_state) reachable_in_approxI_ext:
   assumes monoTyp: "monoTyp typing"
-  and recv_case:
+  and source_case:
     "\<And> t r s i done todo skipped m R step n.
      \<lbrakk> R \<in> P; 
        roleMap r i = Some R;
@@ -588,8 +625,9 @@ lemma (in reachable_state) reachable_in_approxI_ext:
        (t,r,s) \<in> approx typing;
        r i = Some (done, step # todo, skipped);
 
-       recvStep step    \<Longrightarrow> Some m = inst s i (stepPat step) \<and> m \<in> knows t;
-       matchEqStep step \<Longrightarrow> Some (s (matchVar step, i)) = inst s i (stepPat step)
+       recvStep step \<Longrightarrow> Some m = inst s i (stepPat step) \<and> m \<in> knows t;
+       matchEqStep step \<Longrightarrow>
+         the (inst s i (stepPat step)) \<in> typing_A_ext typing (R, matchVar step) i (t,r,s)
      \<rbrakk> \<Longrightarrow> 
         s (MV n i) \<in> typing (R, n) i ( t @ [Step (i, step)], r(i \<mapsto> (done @ [step], todo, skipped)), s)"
   shows "(t,r,s) \<in> approx typing"
@@ -606,7 +644,7 @@ proof(induct rule: reachable_in_approxI[OF monoTyp])
   thus ?case using 1
     apply(subgoal_tac "True")
     apply(clarsimp)
-    apply(rule recv_case)
+    apply(rule source_case)
     by(assumption | simp add: remove_hints)+
 qed
 
